Move wordLang-related syntax lemmas to data_to_wordProof
This is only the first step because many of the lemmas at the
end of data_to_wordProof ought to be moved to the different
word_*Proof theories.

There was one complicated case: assign_get_code_label is a
function over the op datatype from closLang. I didn't know
where to put it so I put it in closLangTheory, because it is
a function directly related to the syntax only. An alternative
would have been to put it in closProps, but that would have
caused bvl, bvi and dataProps to open closProps, which we do
not want for such a simple syntacctic reason.

compiler/backend/proofs/backendProofScript.sml
@@ -147,580 +147,14 @@ val _ = temp_overload_on("stack_remove_prog_comp",``stack_remove$prog_comp``);
 val _ = temp_overload_on("stack_alloc_prog_comp",``stack_alloc$prog_comp``);
 val _ = temp_overload_on("stack_names_prog_comp",``stack_names$prog_comp``);
 
-(* TODO: move things that need moving *)
-
+val _ = temp_overload_on("data_get_code_labels",``dataProps$get_code_labels``);
+val _ = temp_overload_on("data_good_code_labels",``dataProps$good_code_labels``);
 val _ = temp_overload_on("word_get_code_labels",``wordProps$get_code_labels``);
 val _ = temp_overload_on("word_good_handlers",``wordProps$good_handlers``);
 val _ = temp_overload_on("word_good_code_labels",``wordProps$good_code_labels``);
 val _ = temp_overload_on("get_code_labels",``stackProps$get_code_labels``);
 
-(* word_to_word never introduces any labels, so the statements are easy *)
-local
-  open word_removeTheory word_allocTheory word_instTheory word_simpTheory word_to_wordTheory
-  open data_to_wordTheory
-in
-
-(* remove_must_terminate*)
-val word_get_code_labels_remove_must_terminate = Q.prove(`
-  ∀ps.
-  word_get_code_labels (remove_must_terminate ps) =
-  word_get_code_labels ps`,
-  ho_match_mp_tac remove_must_terminate_ind>>rw[]>>
-  fs[remove_must_terminate_def]>>
-  every_case_tac>>fs[]);
-
-val word_good_handlers_remove_must_terminate = Q.prove(`
-  ∀ps.
-  word_good_handlers n (remove_must_terminate ps) ⇔
-  word_good_handlers n ps`,
-  ho_match_mp_tac remove_must_terminate_ind>>rw[]>>
-  fs[remove_must_terminate_def]>>
-  every_case_tac>>fs[]);
-
-(* word_alloc *)
-
-val word_get_code_labels_apply_colour = Q.prove(`
-  ∀col ps.
-  word_get_code_labels (apply_colour col ps) =
-  word_get_code_labels ps`,
-  ho_match_mp_tac apply_colour_ind>>rw[]>>
-  fs[apply_colour_def]>>
-  every_case_tac>>fs[]);
-
-val word_good_handlers_apply_colour = Q.prove(`
-  ∀col ps.
-  word_good_handlers n (apply_colour col ps) ⇔
-  word_good_handlers n ps`,
-  ho_match_mp_tac apply_colour_ind>>rw[]>>
-  fs[apply_colour_def]>>
-  every_case_tac>>fs[]);
-
-val word_get_code_labels_word_alloc = Q.prove(`
-  word_get_code_labels (word_alloc fc c alg k prog col_opt) =
-  word_get_code_labels prog`,
-  fs[word_alloc_def,oracle_colour_ok_def]>>
-  EVERY_CASE_TAC>>fs[]>>
-  TRY(pairarg_tac)>>fs[]>>
-  EVERY_CASE_TAC>>fs[]>>
-  metis_tac[word_get_code_labels_apply_colour])
-
-val word_good_handlers_word_alloc = Q.prove(`
-  word_good_handlers n (word_alloc fc c alg k prog col_opt) ⇔
-  word_good_handlers n prog`,
-  fs[word_alloc_def,oracle_colour_ok_def]>>
-  EVERY_CASE_TAC>>fs[]>>
-  TRY(pairarg_tac)>>fs[]>>
-  EVERY_CASE_TAC>>fs[]>>
-  metis_tac[word_good_handlers_apply_colour]);
-
-(* three to two *)
-val word_get_code_labels_three_to_two_reg = Q.prove(`
-  ∀ps.
-  word_get_code_labels (three_to_two_reg ps) =
-  word_get_code_labels ps`,
-  ho_match_mp_tac three_to_two_reg_ind>>rw[]>>
-  fs[three_to_two_reg_def]>>
-  every_case_tac>>fs[]);
-
-val word_good_handlers_three_to_two_reg = Q.prove(`
-  ∀ps.
-  word_good_handlers n (three_to_two_reg ps) ⇔
-  word_good_handlers n ps`,
-  ho_match_mp_tac three_to_two_reg_ind>>rw[]>>
-  fs[three_to_two_reg_def]>>
-  every_case_tac>>fs[]);
-
-(* remove_dead *)
-val word_get_code_labels_remove_dead = Q.prove(`
-  ∀ps live.
-  word_get_code_labels (FST (remove_dead ps live)) ⊆
-  word_get_code_labels ps`,
-  ho_match_mp_tac remove_dead_ind>>rw[]>>
-  fs[remove_dead_def]>>
-  every_case_tac>>fs[]>>
-  rpt(pairarg_tac>>fs[])>>rw[]>>
-  fs[SUBSET_DEF]);
-
-val word_good_handlers_remove_dead = Q.prove(`
-  ∀ps live.
-  word_good_handlers n ps ⇒
-  word_good_handlers n (FST (remove_dead ps live))`,
-  ho_match_mp_tac remove_dead_ind>>rw[]>>
-  fs[remove_dead_def]>>
-  every_case_tac>>fs[]>>
-  rpt(pairarg_tac>>fs[])>>rw[]);
-
-(* ssa *)
-
-Theorem word_get_code_labels_fake_moves
-  `∀a b c d e f g h i.
-   fake_moves a b c d = (e,f,g,h,i) ⇒
-   word_get_code_labels e = {} ∧
-   word_get_code_labels f = {}`
-  (Induct \\ rw[fake_moves_def] \\ rw[]
-  \\ pairarg_tac \\ fs[]
-  \\ fs[CaseEq"option"] \\ rw[]
-  \\ first_x_assum drule \\ rw[]
-  \\ rw[fake_move_def]);
-
-Theorem word_get_code_labels_ssa_cc_trans
-  `∀x y z a b c.
-   ssa_cc_trans x y z = (a,b,c) ⇒
-   word_get_code_labels a = word_get_code_labels x`
-  (recInduct ssa_cc_trans_ind
-  \\ rw[ssa_cc_trans_def] \\ fs[]
-  \\ rpt(pairarg_tac \\ fs[]) \\ rveq \\ fs[]
-  >- (
-    Cases_on`i` \\ fs[ssa_cc_trans_inst_def]
-    \\ rveq \\ fs[]
-    \\ rpt(pairarg_tac \\ fs[]) \\ rveq \\ fs[]
-    \\ TRY(rename1`Arith arith` \\ Cases_on`arith`)
-    \\ TRY(rename1`Mem memop _ dst` \\ Cases_on`memop` \\ Cases_on`dst`)
-    \\ TRY(rename1`FP flop` \\ Cases_on`flop`)
-    \\ fs[ssa_cc_trans_inst_def,CaseEq"reg_imm",CaseEq"bool"]
-    \\ rpt(pairarg_tac \\ fs[]) \\ rveq \\ fs[] )
-  >- (
-    fs[fix_inconsistencies_def]
-    \\ rpt(pairarg_tac \\ fs[])
-    \\ rveq \\ fs[]
-    \\ imp_res_tac word_get_code_labels_fake_moves
-    \\ rw[])
-  >- (
-    fs[list_next_var_rename_move_def]
-    \\ rpt(pairarg_tac \\ fs[])
-    \\ rveq \\ fs[] )
-  >- (
-    fs[list_next_var_rename_move_def]
-    \\ rpt(pairarg_tac \\ fs[])
-    \\ rveq \\ fs[] )
-  >- (
-    fs[list_next_var_rename_move_def]
-    \\ rpt(pairarg_tac \\ fs[])
-    \\ rveq \\ fs[] )
-  >- (
-    fs[CaseEq"option"] \\ rveq \\ fs[]
-    \\ fs[list_next_var_rename_move_def]
-    \\ rpt(pairarg_tac \\ fs[])
-    \\ rveq \\ fs[]
-    \\ fs[CaseEq"prod", fix_inconsistencies_def]
-    \\ rpt(pairarg_tac \\ fs[])
-    \\ rveq \\ fs[]
-    \\ imp_res_tac word_get_code_labels_fake_moves
-    \\ fs[]));
-
-val word_get_code_labels_full_ssa_cc_trans = Q.prove(`
-  ∀m p.
-  word_get_code_labels (full_ssa_cc_trans m p) =
-  word_get_code_labels p`,
-  simp[full_ssa_cc_trans_def]
-  \\ rpt gen_tac
-  \\ pairarg_tac \\ fs[]
-  \\ pairarg_tac \\ fs[]
-  \\ fs[setup_ssa_def]
-  \\ pairarg_tac \\ fs[]
-  \\ rveq \\ fs[]
-  \\ drule word_get_code_labels_ssa_cc_trans
-  \\ rw[]);
-
-Theorem word_good_handlers_fake_moves
-  `∀a b c d e f g h i.
-   fake_moves a b c d = (e,f,g,h,i) ⇒
-   word_good_handlers n e ∧
-   word_good_handlers n f`
-  (Induct \\ rw[fake_moves_def] \\ rw[]
-  \\ pairarg_tac \\ fs[]
-  \\ fs[CaseEq"option"] \\ rw[]
-  \\ first_x_assum drule \\ rw[]
-  \\ rw[fake_move_def]);
-
-Theorem word_good_handlers_ssa_cc_trans
-  `∀x y z a b c.
-   ssa_cc_trans x y z = (a,b,c) ⇒
-   word_good_handlers n a = word_good_handlers n x`
-  (recInduct ssa_cc_trans_ind
-  \\ rw[ssa_cc_trans_def] \\ fs[]
-  \\ rpt(pairarg_tac \\ fs[]) \\ rveq \\ fs[]
-  >- (
-    Cases_on`i` \\ fs[ssa_cc_trans_inst_def]
-    \\ rveq \\ fs[]
-    \\ rpt(pairarg_tac \\ fs[]) \\ rveq \\ fs[]
-    \\ TRY(rename1`Arith arith` \\ Cases_on`arith`)
-    \\ TRY(rename1`Mem memop _ dst` \\ Cases_on`memop` \\ Cases_on`dst`)
-    \\ TRY(rename1`FP flop` \\ Cases_on`flop`)
-    \\ fs[ssa_cc_trans_inst_def,CaseEq"reg_imm",CaseEq"bool"]
-    \\ rpt(pairarg_tac \\ fs[]) \\ rveq \\ fs[] )
-  >- (
-    fs[fix_inconsistencies_def]
-    \\ rpt(pairarg_tac \\ fs[])
-    \\ rveq \\ fs[]
-    \\ imp_res_tac word_good_handlers_fake_moves
-    \\ rw[])
-  >- (
-    fs[list_next_var_rename_move_def]
-    \\ rpt(pairarg_tac \\ fs[])
-    \\ rveq \\ fs[] )
-  >- (
-    fs[list_next_var_rename_move_def]
-    \\ rpt(pairarg_tac \\ fs[])
-    \\ rveq \\ fs[] )
-  >- (
-    fs[list_next_var_rename_move_def]
-    \\ rpt(pairarg_tac \\ fs[])
-    \\ rveq \\ fs[] )
-  >- (
-    fs[CaseEq"option"] \\ rveq \\ fs[]
-    \\ fs[list_next_var_rename_move_def]
-    \\ rpt(pairarg_tac \\ fs[])
-    \\ rveq \\ fs[]
-    \\ fs[CaseEq"prod", fix_inconsistencies_def]
-    \\ rpt(pairarg_tac \\ fs[])
-    \\ rveq \\ fs[]
-    \\ imp_res_tac word_good_handlers_fake_moves
-    \\ fs[]));
-
-val word_good_handlers_full_ssa_cc_trans = Q.prove(`
-  ∀m p.
-  word_good_handlers n (full_ssa_cc_trans m p) ⇔
-  word_good_handlers n p`,
-  simp[full_ssa_cc_trans_def]
-  \\ rpt gen_tac
-  \\ pairarg_tac \\ fs[]
-  \\ pairarg_tac \\ fs[]
-  \\ fs[setup_ssa_def]
-  \\ pairarg_tac \\ fs[]
-  \\ rveq \\ fs[]
-  \\ drule word_good_handlers_ssa_cc_trans
-  \\ rw[]);
-
-(* inst *)
-val word_get_code_labels_inst_select_exp = Q.prove(`
-  ∀a b c exp.
-  word_get_code_labels (inst_select_exp a b c exp) = {}`,
-  ho_match_mp_tac inst_select_exp_ind>>rw[]>>
-  fs[inst_select_exp_def]>>
-  every_case_tac>>fs[inst_select_exp_def]);
-
-val word_get_code_labels_inst_select = Q.prove(`
-  ∀ac v ps.
-  word_get_code_labels (inst_select ac v ps) =
-  word_get_code_labels ps`,
-  ho_match_mp_tac inst_select_ind>>rw[]>>
-  fs[inst_select_def]>>
-  every_case_tac>>fs[word_get_code_labels_inst_select_exp]);
-
-val word_good_handlers_inst_select_exp = Q.prove(`
-  ∀a b c exp.
-  word_good_handlers n (inst_select_exp a b c exp)`,
-  ho_match_mp_tac inst_select_exp_ind>>rw[]>>
-  fs[inst_select_exp_def]>>
-  every_case_tac>>fs[inst_select_exp_def]);
-
-val word_good_handlers_inst_select = Q.prove(`
-  ∀ac v ps.
-  word_good_handlers n (inst_select ac v ps) ⇔
-  word_good_handlers n ps`,
-  ho_match_mp_tac inst_select_ind>>rw[]>>
-  fs[inst_select_def]>>
-  every_case_tac>>fs[word_good_handlers_inst_select_exp]);
-
-(* simp *)
-val word_get_code_labels_const_fp_loop = Q.prove(`
-  ∀p l.
-  word_get_code_labels (FST (const_fp_loop p l)) ⊆ word_get_code_labels p`,
-  ho_match_mp_tac const_fp_loop_ind \\ rw []
-  \\ fs [const_fp_loop_def]
-  \\ every_case_tac\\ fs[]
-  \\ rpt (pairarg_tac \\ fs[])
-  \\ fs[SUBSET_DEF] \\ metis_tac[]);
-
-val word_good_handlers_const_fp_loop = Q.prove(`
-  ∀p l.
-  word_good_handlers n p ⇒
-  word_good_handlers n (FST (const_fp_loop p l))`,
-  ho_match_mp_tac const_fp_loop_ind \\ rw []
-  \\ fs [const_fp_loop_def]
-  \\ every_case_tac\\ fs[]
-  \\ rpt (pairarg_tac \\ fs[]));
-
-Theorem word_get_code_labels_apply_if_opt
-  `∀x y z. apply_if_opt x y = SOME z ⇒ word_get_code_labels z = word_get_code_labels x ∪ word_get_code_labels y`
-  (rw[apply_if_opt_def]
-  \\ fs[CaseEq"option",CaseEq"prod"]
-  \\ pairarg_tac \\ fs[]
-  \\ fs[CaseEq"option",CaseEq"prod"]
-  \\ rveq
-  \\ fs[CaseEq"bool"] \\ rveq
-  \\ rw[SmartSeq_def]
-  \\ rename1`dest_If iff`
-  \\ Cases_on`iff` \\ fs[dest_If_def]
-  \\ rveq \\ fs[]
-  \\ fs[dest_If_Eq_Imm_def,CaseEq"option",CaseEq"prod",CaseEq"cmp",CaseEq"reg_imm"]
-  \\ Cases_on`y` \\ fs[dest_If_def] \\ rveq
-  \\ Cases_on`x` \\ fs[dest_Seq_def] \\ rveq \\ fs[]
-  \\ rw[EXTENSION, EQ_IMP_THM] \\ rw[]);
-
-Theorem word_get_code_labels_simp_if[simp]
-   `∀p.  word_get_code_labels (simp_if p) = word_get_code_labels p`
-  (recInduct simp_if_ind
-  \\ rw[simp_if_def]
-  \\ CASE_TAC \\ simp[]
-  >- ( drule word_get_code_labels_apply_if_opt \\ rw[] )
-  \\ every_case_tac \\ fs[]);
-
-Theorem word_good_handlers_apply_if_opt
-  `∀x y z. apply_if_opt x y = SOME z ∧
-           word_good_handlers n x ∧ word_good_handlers n y
-           ⇒
-           word_good_handlers n z `
-  (rw[apply_if_opt_def]
-  \\ fs[CaseEq"option",CaseEq"prod"]
-  \\ pairarg_tac \\ fs[]
-  \\ fs[CaseEq"option",CaseEq"prod"]
-  \\ rveq
-  \\ fs[CaseEq"bool"] \\ rveq
-  \\ rw[SmartSeq_def]
-  \\ rename1`dest_If iff`
-  \\ Cases_on`iff` \\ fs[dest_If_def]
-  \\ rveq \\ fs[]
-  \\ fs[dest_If_Eq_Imm_def,CaseEq"option",CaseEq"prod",CaseEq"cmp",CaseEq"reg_imm"]
-  \\ Cases_on`y` \\ fs[dest_If_def] \\ rveq
-  \\ Cases_on`x` \\ fs[dest_Seq_def] \\ rveq \\ fs[]);
-
-val word_good_handlers_simp_if = Q.prove(`
-  ∀p.
-  word_good_handlers n p ⇒
-  word_good_handlers n (simp_if p)`,
-  recInduct simp_if_ind
-  \\ rw[simp_if_def]
-  \\ CASE_TAC \\ simp[]
-  >- ( drule word_good_handlers_apply_if_opt \\ rw[] )
-  \\ every_case_tac \\ fs[]);
-
-val word_get_code_labels_Seq_assoc = Q.prove(`
-  ∀p1 p2.
-  word_get_code_labels (Seq_assoc p1 p2) = word_get_code_labels p1 ∪ word_get_code_labels p2`,
-  ho_match_mp_tac Seq_assoc_ind>>rw[]>>
-  fs[Seq_assoc_def,SmartSeq_def]>>rw[]>>
-  fs[UNION_ASSOC]>>
-  every_case_tac>>fs[]);
-
-val word_good_handlers_Seq_assoc = Q.prove(`
-  ∀p1 p2.
-  word_good_handlers n (Seq_assoc p1 p2) ⇔
-  word_good_handlers n p1 ∧ word_good_handlers n p2`,
-  ho_match_mp_tac Seq_assoc_ind>>rw[]>>
-  fs[Seq_assoc_def,SmartSeq_def]>>rw[]>>
-  every_case_tac>>fs[]>>metis_tac[]);
-
-val word_get_code_labels_word_simp = Q.prove(`
-  ∀ps.
-  word_get_code_labels (word_simp$compile_exp ps) ⊆
-  word_get_code_labels ps`,
-  PURE_REWRITE_TAC [compile_exp_def]>>
-  LET_ELIM_TAC>>
-  match_mp_tac SUBSET_TRANS >>
-  qexists_tac`word_get_code_labels e'`>>rw[]
-  >- (
-    unabbrev_all_tac>>EVAL_TAC>>
-    metis_tac[word_get_code_labels_const_fp_loop])>>
-  match_mp_tac SUBSET_TRANS >>
-  qexists_tac`word_get_code_labels e`>>rw[]
-  >- (
-    unabbrev_all_tac>>EVAL_TAC>>
-    metis_tac[word_get_code_labels_simp_if, SUBSET_REFL])>>
-  unabbrev_all_tac>>
-  fs[word_get_code_labels_Seq_assoc]);
-
-val word_good_handlers_word_simp = Q.prove(`
-  ∀ps.
-  word_good_handlers n ps ⇒
-  word_good_handlers n (word_simp$compile_exp ps)`,
-  rw[compile_exp_def]>>
-  EVAL_TAC>>match_mp_tac word_good_handlers_const_fp_loop>>
-  match_mp_tac word_good_handlers_simp_if>>
-  fs[word_good_handlers_Seq_assoc]);
-
-val word_get_code_labels_word_to_word = Q.prove(`
-  word_good_code_labels progs ⇒
-  word_good_code_labels (SND (compile wc ac progs))`,
-  fs[word_to_wordTheory.compile_def]>>
-  rpt(pairarg_tac>>fs[])>>
-  fs[wordPropsTheory.good_code_labels_def,next_n_oracle_def]>>
-  rw[]
-  >- (
-    rfs[EVERY_MAP,LENGTH_GENLIST,EVERY_MEM,MEM_ZIP,PULL_EXISTS]>>
-    rw[full_compile_single_def]>>
-    Cases_on`EL n progs`>>Cases_on`r`>>fs[compile_single_def]>>
-    fs[word_good_handlers_remove_must_terminate,word_good_handlers_word_alloc]>>
-    simp[COND_RAND]>>
-    fs[word_good_handlers_three_to_two_reg]>>
-    match_mp_tac word_good_handlers_remove_dead>>
-    simp[word_good_handlers_full_ssa_cc_trans,word_good_handlers_inst_select]>>
-    match_mp_tac word_good_handlers_word_simp>>
-    fs[FORALL_PROD]>>
-    metis_tac[EL_MEM])
-  >>
-    fs[SUBSET_DEF,PULL_EXISTS,MEM_MAP,MEM_ZIP]>>
-    rw[full_compile_single_def]>>
-    Cases_on`EL n progs`>>Cases_on`r`>>fs[compile_single_def]>>
-    fs[word_get_code_labels_remove_must_terminate,word_get_code_labels_word_alloc]>>
-    fs[COND_RAND]>>
-    fs[word_get_code_labels_three_to_two_reg]>>
-    drule (word_get_code_labels_remove_dead|>SIMP_RULE std_ss [SUBSET_DEF])>>
-    simp[word_get_code_labels_full_ssa_cc_trans,word_get_code_labels_inst_select]>>
-    strip_tac>>
-    drule (word_get_code_labels_word_simp|>SIMP_RULE std_ss [SUBSET_DEF])>>
-    rw[]>>fs[FORALL_PROD,EXISTS_PROD,PULL_EXISTS,EVERY_MEM]>>
-    first_x_assum drule>>
-    disch_then(qspecl_then [`q`,`q'`] mp_tac)>>
-    impl_tac >-
-        metis_tac[EL_MEM]>>
-    rw[]>>
-    fs[MEM_EL]>>
-    qexists_tac`n'`>>simp[]>>
-    Cases_on`EL n' progs`>>Cases_on`r`>>fs[compile_single_def]);
-
-val assign_get_code_label_def = Define`
-  (assign_get_code_label (closLang$Label x) = {x}) ∧
-  (assign_get_code_label x = {})`
-
-val data_get_code_labels_def = Define`
-  (data_get_code_labels (Call r d a h) =
-    (case d of SOME x => {x} | _ => {}) ∪
-    (case h of SOME (n,p) => data_get_code_labels p | _ => {})) ∧
-  (data_get_code_labels (Seq p1 p2) = data_get_code_labels p1 ∪ data_get_code_labels p2) ∧
-  (data_get_code_labels (If _ p1 p2) = data_get_code_labels p1 ∪ data_get_code_labels p2) ∧
-  (data_get_code_labels (Assign _ op _ _) = assign_get_code_label op) ∧
-  (data_get_code_labels _ = {})`;
-val _ = export_rewrites["data_get_code_labels_def"];
-
-val word_get_code_labels_StoreEach = Q.prove(`
-  ∀ls off.
-  word_get_code_labels (StoreEach v ls off) = {}`,
-  Induct>>fs[StoreEach_def]);
-
-val word_get_code_labels_MemEqList = Q.prove(`
-  ∀x b.
-  word_get_code_labels (MemEqList b x) = {}`,
-  Induct>>fs[MemEqList_def]);
-
-(* slow... *)
-val word_get_code_labels_assign = Q.prove(`
-  ∀x.
-  word_get_code_labels (FST (assign c secn v w x y z)) SUBSET
-  assign_get_code_label x ∪ (set(MAP FST (stubs (:α) c)))`,
-  ho_match_mp_tac (fetch "-" "assign_get_code_label_ind")>>
-  rw[assign_def,all_assign_defs,arg1_def,arg2_def,arg3_def,arg4_def,
-     assign_get_code_label_def]>>
-  fs[list_Seq_def,word_get_code_labels_StoreEach,word_get_code_labels_MemEqList]>>
-  rpt(every_case_tac>>fs[]>>
-  fs[list_Seq_def,word_get_code_labels_StoreEach,word_get_code_labels_MemEqList]>>
-  EVAL_TAC));
-
-val data_to_word_comp_code_labels = Q.prove(`
-  ∀c secn l p.
-  word_get_code_labels ((FST (comp c secn l p)):'a wordLang$prog) SUBSET
-  data_get_code_labels p ∪ set(MAP FST (stubs (:α) c))`,
-  ho_match_mp_tac comp_ind>>
-  rw[]>>Cases_on`p`>>fs[]>>
-  simp[Once comp_def]>>
-  rpt(pairarg_tac>>fs[])
-  >- (
-    every_case_tac>>fs[]>>
-    rpt(pairarg_tac>>fs[])>>
-    fs[SUBSET_DEF]>>fs[]>>
-    metis_tac[])
-  >-
-    fs[word_get_code_labels_assign]
-  >-
-    (fs[SUBSET_DEF]>>metis_tac[])
-  >-
-    (fs[SUBSET_DEF]>>metis_tac[])
-  >>
-    EVAL_TAC>>rw[]>>fs[]);
-
-val word_good_handlers_StoreEach = Q.prove(`
-  ∀ls off.
-  word_good_handlers secn (StoreEach v ls off)`,
-  Induct>>fs[StoreEach_def]);
-
-val word_good_handlers_MemEqList = Q.prove(`
-  ∀x b.
-  word_good_handlers secn (MemEqList b x)`,
-  Induct>>fs[MemEqList_def]);
-
-(* slow... *)
-val word_good_handlers_assign = Q.prove(`
-  ∀x.
-  word_good_handlers secn (FST (assign c secn v w x y z))`,
-  ho_match_mp_tac (fetch "-" "assign_get_code_label_ind")>>
-  rw[assign_def,all_assign_defs,arg1_def,arg2_def,arg3_def,arg4_def]>>
-  rpt(
-  every_case_tac>>fs[list_Seq_def,word_good_handlers_StoreEach,word_good_handlers_MemEqList]>>
-  rw[]>>EVAL_TAC
-  ));
-
-val data_to_word_comp_good_handlers = Q.prove(`
-  ∀c secn l p.
-  word_good_handlers secn ((FST (comp c secn l p)):'a wordLang$prog)`,
-  ho_match_mp_tac comp_ind>>
-  rw[]>>Cases_on`p`>>fs[]>>
-  simp[Once comp_def]>>
-  rpt(pairarg_tac>>fs[])
-  >- (
-    every_case_tac>>fs[]>>
-    rpt(pairarg_tac>>fs[])>>
-    fs[SUBSET_DEF]>>fs[]>>
-    metis_tac[])
-  >-
-    fs[word_good_handlers_assign]
-  >>
-    EVAL_TAC>>rw[]>>fs[]);
-
-val data_good_code_labels_def = Define`
-  data_good_code_labels p ⇔
-  (BIGUNION (set (MAP (λ(n,m,pp). (data_get_code_labels pp)) p))) ⊆
-  (set (MAP FST p))`
-
-val stubs_labels = Q.prove(`
-  BIGUNION (set (MAP (λ(n,m,pp). word_get_code_labels pp)  (stubs (:'a) data_conf)))
-  ⊆ set (MAP FST (stubs (:'a) data_conf))`,
-  rpt(EVAL_TAC>>
-  IF_CASES_TAC>>
-  simp[]));
-
-Theorem data_to_word_good_code_labels `
-  (data_to_word$compile data_conf word_conf asm_conf prog) = (xx,prog') ∧
-  data_good_code_labels prog ⇒
-  word_good_code_labels prog'`
-  (fs[data_to_wordTheory.compile_def]>>rw[]>>
-  qmatch_asmsub_abbrev_tac`LHS = _`>>
-  `prog' = SND LHS` by (unabbrev_all_tac>>fs[])>>
-  pop_assum SUBST_ALL_TAC>>
-  fs[Abbr`LHS`]>>
-  match_mp_tac word_get_code_labels_word_to_word>>
-  fs[wordPropsTheory.good_code_labels_def,data_good_code_labels_def]>>rw[]
-  >-
-    (EVAL_TAC>>rw[])
-  >-
-    (simp[EVERY_MAP,LAMBDA_PROD,compile_part_def,data_to_word_comp_good_handlers]>>
-    fs[EVERY_MEM,FORALL_PROD])
-  >-
-    (assume_tac stubs_labels>>
-    match_mp_tac SUBSET_TRANS>>asm_exists_tac>>fs[])
-  >>
-    fs[MAP_MAP_o,o_DEF,LAMBDA_PROD,compile_part_def]>>
-    fs[SUBSET_DEF,PULL_EXISTS,Once MEM_MAP,FORALL_PROD]>>
-    rw[]>>
-    drule (data_to_word_comp_code_labels |> SIMP_RULE std_ss [SUBSET_DEF])>>
-    rw[]
-    >-
-      (first_x_assum drule>>
-      disch_then drule>>fs[MEM_MAP,EXISTS_PROD])
-    >>
-      fs[MEM_MAP]>>metis_tac[]);
-
-end
+(* TODO: move things that need moving *)
 
 Theorem compile_prog_keeps_names
   `∀next xs next' ys. compile_prog next xs = (next',ys) ∧ MEM x (MAP FST xs) ⇒ MEM x (MAP FST ys)`
@@ -730,14 +164,14 @@ Theorem compile_prog_keeps_names
   \\ fs[CaseEq"option",CaseEq"prod"] \\ rveq \\ fs[]);
 
 val bvl_get_code_labels_def = tDefine"bvl_get_code_labels"
-  `(bvl_get_code_labels (Var _) = {}) ∧
+  `(bvl_get_code_labels (bvl$Var _) = {}) ∧
    (bvl_get_code_labels (If e1 e2 e3) = bvl_get_code_labels e1 ∪ bvl_get_code_labels e2 ∪ bvl_get_code_labels e3) ∧
    (bvl_get_code_labels (Let es e) = BIGUNION (set (MAP bvl_get_code_labels es)) ∪ bvl_get_code_labels e) ∧
    (bvl_get_code_labels (Raise e) = bvl_get_code_labels e) ∧
    (bvl_get_code_labels (Handle e1 e2) = bvl_get_code_labels e1 ∪ bvl_get_code_labels e2) ∧
    (bvl_get_code_labels (Tick e) = bvl_get_code_labels e) ∧
    (bvl_get_code_labels (Call _ d es) = (case d of NONE => {} | SOME n => {n}) ∪ BIGUNION (set (MAP bvl_get_code_labels es))) ∧
-   (bvl_get_code_labels (Op op es) = assign_get_code_label op ∪ BIGUNION (set (MAP bvl_get_code_labels es)))`
+   (bvl_get_code_labels (Op op es) = closLang$assign_get_code_label op ∪ BIGUNION (set (MAP bvl_get_code_labels es)))`
   (wf_rel_tac`measure exp_size`
    \\ simp[bvlTheory.exp_size_def]
    \\ rpt conj_tac \\ rpt gen_tac
@@ -760,7 +194,7 @@ val bvi_get_code_labels_def = tDefine"bvi_get_code_labels"
      (case d of NONE => {} | SOME n => {n}) ∪
      (case h of NONE => {} | SOME e => bvi_get_code_labels e) ∪
      BIGUNION (set (MAP bvi_get_code_labels es))) ∧
-   (bvi_get_code_labels (Op op es) = assign_get_code_label op ∪ BIGUNION (set (MAP bvi_get_code_labels es)))`
+   (bvi_get_code_labels (Op op es) = closLang$assign_get_code_label op ∪ BIGUNION (set (MAP bvi_get_code_labels es)))`
   (wf_rel_tac`measure exp_size`
    \\ simp[bviTheory.exp_size_def]
    \\ rpt conj_tac \\ rpt gen_tac
@@ -821,7 +255,7 @@ Theorem data_get_code_labels_mk_ticks
    \\ rw[]);
 
 Theorem data_get_code_labels_iAssign[simp]
-  `∀a b c d e. data_get_code_labels (iAssign a b c d e) = assign_get_code_label b`
+  `∀a b c d e. data_get_code_labels (iAssign a b c d e) = closLang$assign_get_code_label b`
   (rw[bvi_to_dataTheory.iAssign_def]
   \\ EVAL_TAC);
 
@@ -845,7 +279,7 @@ Theorem data_get_code_labels_compile_TODO_move2
 Theorem compile_prog_good_code_labels
   `∀p. bvi_good_code_labels p ⇒ data_good_code_labels (bvi_to_data$compile_prog p)`
   (simp[bvi_to_dataTheory.compile_prog_def]
-  \\ simp[data_good_code_labels_def, MAP_MAP_o, o_DEF, LAMBDA_PROD]
+  \\ simp[dataPropsTheory.good_code_labels_def, MAP_MAP_o, o_DEF, LAMBDA_PROD]
   \\ simp[bvi_to_dataTheory.compile_part_def]
   \\ simp[FST_triple]
   \\ simp[bvi_good_code_labels_def]
@@ -881,7 +315,7 @@ Theorem bvi_get_code_labels_rewrite
   \\ fs[CaseEq"option"] \\ rveq
   \\ fs[bvi_tailrecTheory.check_op_def,CaseEq"option",CaseEq"prod",CaseEq"bool"] \\ rveq \\ fs[]
   \\ rveq \\ fs[bvi_tailrecTheory.apply_op_def] \\ rw[] \\ fs[SUBSET_DEF]
-  \\ Cases_on`opr` \\ fs[bvi_tailrecTheory.to_op_def, assign_get_code_label_def]
+  \\ Cases_on`opr` \\ fs[bvi_tailrecTheory.to_op_def, closLangTheory.assign_get_code_label_def]
   \\ fs[bvi_tailrecTheory.opbinargs_def, bvi_tailrecTheory.get_bin_args_def]
   \\ imp_res_tac bvi_tailrecProofTheory.is_rec_term_ok \\ fs[]
   \\ TRY(metis_tac[])
@@ -889,11 +323,11 @@ Theorem bvi_get_code_labels_rewrite
   \\ rename1`Call _ opt _ _`
   \\ Cases_on`opt` \\ fs[bvi_tailrecTheory.is_rec_def]
   \\ fs[bvi_tailrecTheory.args_from_def,bvi_tailrecTheory.push_call_def]
-  \\ fs[bvi_tailrecTheory.apply_op_def, bvi_tailrecTheory.to_op_def, assign_get_code_label_def]
+  \\ fs[bvi_tailrecTheory.apply_op_def, bvi_tailrecTheory.to_op_def, closLangTheory.assign_get_code_label_def]
   \\ fs[bvi_tailrecTheory.try_swap_def, bvi_tailrecTheory.opbinargs_def]
   \\ fs[CaseEq"bool",CaseEq"option"] \\ rveq
   \\ fs[CaseEq"option",bvi_tailrecTheory.get_bin_args_def,CaseEq"bool",bvi_tailrecTheory.apply_op_def] \\ rveq \\ fs[]
-  \\ fs[PULL_EXISTS, assign_get_code_label_def]
+  \\ fs[PULL_EXISTS, closLangTheory.assign_get_code_label_def]
   \\ TRY(EVAL_TAC \\ rw[] \\ NO_TAC)
   \\ fsrw_tac[DNF_ss][PULL_EXISTS]
   \\ metis_tac[]);
@@ -913,7 +347,7 @@ Theorem bvi_get_code_labels_compile_exp
   \\ pairarg_tac \\ fs[] \\ rveq
   \\ drule bvi_get_code_labels_rewrite
   \\ simp[] \\ strip_tac
-  \\ Cases_on`op` \\ simp[bvi_tailrecTheory.id_from_op_def, assign_get_code_label_def]
+  \\ Cases_on`op` \\ simp[bvi_tailrecTheory.id_from_op_def, closLangTheory.assign_get_code_label_def]
   \\ EVAL_TAC);
 
 Theorem TODO_MOVE_1_compile_prog_good_code_labels
@@ -985,15 +419,15 @@ Theorem compile_int_code_labels[simp]
   (recInduct bvl_to_bviTheory.compile_int_ind
   \\ rw[]
   \\ rw[Once bvl_to_bviTheory.compile_int_def]
-  \\ rw[assign_get_code_label_def]);
+  \\ rw[closLangTheory.assign_get_code_label_def]);
 
 Theorem compile_op_code_labels
   `bvi_get_code_labels (compile_op op c) ⊆
     BIGUNION (set (MAP bvi_get_code_labels c)) ∪
-    IMAGE (λn. bvl_num_stubs + n * bvl_to_bvi_namespaces) (assign_get_code_label op) ∪
+    IMAGE (λn. bvl_num_stubs + n * bvl_to_bvi_namespaces) (closLang$assign_get_code_label op) ∪
     set (MAP FST (bvl_to_bvi$stubs x y))`
   (simp[bvl_to_bviTheory.compile_op_def, bvl_to_bviTheory.stubs_def, SUBSET_DEF]
-  \\ every_case_tac \\ fs[assign_get_code_label_def, REPLICATE_GENLIST, PULL_EXISTS, MAPi_GENLIST, MEM_GENLIST]
+  \\ every_case_tac \\ fs[closLangTheory.assign_get_code_label_def, REPLICATE_GENLIST, PULL_EXISTS, MAPi_GENLIST, MEM_GENLIST]
   \\ rw[] \\ fsrw_tac[DNF_ss][PULL_EXISTS] \\ metis_tac[]);
 
 Theorem dest_var_code_labels[simp]
@@ -1298,16 +732,16 @@ Theorem dest_simple_SOME_code_labels
 
 Theorem SmartOp2_code_labels[simp]
   `bvl_get_code_labels (SmartOp2 (op,x1,x2)) =
-    assign_get_code_label op ∪ bvl_get_code_labels x1 ∪ bvl_get_code_labels x2`
-  (rw[bvl_constTheory.SmartOp2_def, assign_get_code_label_def]
-  \\ rpt(PURE_CASE_TAC \\ simp[assign_get_code_label_def])
+    closLang$assign_get_code_label op ∪ bvl_get_code_labels x1 ∪ bvl_get_code_labels x2`
+  (rw[bvl_constTheory.SmartOp2_def, closLangTheory.assign_get_code_label_def]
+  \\ rpt(PURE_CASE_TAC \\ simp[closLangTheory.assign_get_code_label_def])
   \\ imp_res_tac dest_simple_SOME_code_labels \\ fs[]
   \\ fs[bvl_constTheory.case_op_const_def, CaseEq"option", CaseEq"closLang$op", CaseEq"bvl$exp", CaseEq"list", NULL_EQ]
-  \\ rveq \\ fs[assign_get_code_label_def,bvlTheory.Bool_def]
+  \\ rveq \\ fs[closLangTheory.assign_get_code_label_def,bvlTheory.Bool_def]
   \\ simp[EXTENSION] \\ metis_tac[]);
 
 Theorem SmartOp_code_labels[simp]
-  `bvl_get_code_labels (SmartOp op xs) = assign_get_code_label op ∪ BIGUNION (set (MAP bvl_get_code_labels xs))`
+  `bvl_get_code_labels (SmartOp op xs) = closLang$assign_get_code_label op ∪ BIGUNION (set (MAP bvl_get_code_labels xs))`
   (rw[bvl_constTheory.SmartOp_def]
   \\ PURE_CASE_TAC \\ simp[]
   \\ PURE_CASE_TAC \\ simp[]
@@ -1316,7 +750,7 @@ Theorem SmartOp_code_labels[simp]
   \\ PURE_TOP_CASE_TAC \\ fs[]
   >- ( rw[EXTENSION] \\ metis_tac[] )
   \\ imp_res_tac dest_simple_SOME_code_labels
-  \\ rw[assign_get_code_label_def]);
+  \\ rw[closLangTheory.assign_get_code_label_def]);
 
 Theorem MEM_extract_list_code_labels
   `∀xs x. MEM (SOME x) (extract_list xs) ⇒ bvl_get_code_labels x = {}`
@@ -1472,7 +906,7 @@ Theorem tick_inline_code_labels
     \\ fs [bvl_inlineTheory.LENGTH_tick_inline] \\ rw []
     \\ fs [SUBSET_DEF] \\ rw [] \\ metis_tac [])
   \\ TRY
-   (rename1 `assign_get_code_label op`
+   (rename1 `closLang$assign_get_code_label op`
     \\ fs [SUBSET_DEF] \\ rw [] \\ metis_tac [])
   \\ TRY (* what... *)
    (rename1 `option_CASE dest`
@@ -1537,8 +971,8 @@ Theorem set_MAP_code_sort
   \\ imp_res_tac MEM_PERM \\ fs[]);
 
 Theorem assign_get_code_label_compile_op
-  `assign_get_code_label (compile_op op) = case some n. op = Label n of SOME n => {n} | _ => {}`
-  (Cases_on`op` \\ rw[clos_to_bvlTheory.compile_op_def, assign_get_code_label_def]);
+  `closLang$assign_get_code_label (compile_op op) = case some n. op = Label n of SOME n => {n} | _ => {}`
+  (Cases_on`op` \\ rw[clos_to_bvlTheory.compile_op_def, closLangTheory.assign_get_code_label_def]);
 
 val clos_get_code_labels_def = tDefine"bvl_get_code_labels" `
   (clos_get_code_labels (Var _ _) = {}) ∧
@@ -1570,7 +1004,7 @@ val clos_get_code_labels_def = tDefine"bvl_get_code_labels" `
     BIGUNION (set (MAP clos_get_code_labels (MAP SND es)))) ∧
   (clos_get_code_labels (Op _ op es) =
     BIGUNION (set (MAP clos_get_code_labels es)) ∪
-    assign_get_code_label op)`
+    closLang$assign_get_code_label op)`
   (wf_rel_tac `measure exp_size`
    \\ simp [closLangTheory.exp_size_def]
    \\ rpt conj_tac \\ rpt gen_tac
@@ -1596,7 +1030,7 @@ Theorem recc_Lets_code_labels
    IMAGE (λj. n + 2 * j) (count k) ∪ bvl_get_code_labels rest`
   (recInduct clos_to_bvlTheory.recc_Lets_ind \\ rw[]
   \\ rw[Once clos_to_bvlTheory.recc_Lets_def] \\ fs[]
-  \\ fs[clos_to_bvlTheory.recc_Let_def, assign_get_code_label_def]
+  \\ fs[clos_to_bvlTheory.recc_Let_def, closLangTheory.assign_get_code_label_def]
   \\ rw[Once EXTENSION]
   \\ Cases_on`k` \\ fs[]
   \\ fsrw_tac[DNF_ss][EQ_IMP_THM, PULL_EXISTS,ADD1] \\ rw[ADD1]
@@ -1626,12 +1060,12 @@ Theorem compile_exps_code_labels
   \\ rw [clos_to_bvlTheory.compile_exps_def] \\ rw []
   \\ rpt (pairarg_tac \\ fs []) \\ rw []
   \\ imp_res_tac clos_to_bvlTheory.compile_exps_SING \\ rveq \\ fs []
-  \\ fs[assign_get_code_label_def]
+  \\ fs[closLangTheory.assign_get_code_label_def]
   \\ fs[MAP_GENLIST, o_DEF]
   \\ TRY (
     CHANGED_TAC(rw[assign_get_code_label_compile_op])
     \\ CASE_TAC \\ fs[]
-    \\ Cases_on`op` \\ fs[assign_get_code_label_def]
+    \\ Cases_on`op` \\ fs[closLangTheory.assign_get_code_label_def]
     \\ fsrw_tac[DNF_ss][]
     \\ NO_TAC )
   \\ TRY (
@@ -1640,7 +1074,7 @@ Theorem compile_exps_code_labels
     \\ metis_tac[] )
   \\ TRY (
     reverse PURE_CASE_TAC
-    \\ fs[clos_to_bvlTheory.mk_cl_call_def, assign_get_code_label_def, MAP_GENLIST, o_DEF]
+    \\ fs[clos_to_bvlTheory.mk_cl_call_def, closLangTheory.assign_get_code_label_def, MAP_GENLIST, o_DEF]
     \\ fs[SUBSET_DEF, PULL_EXISTS, MEM_GENLIST, clos_to_bvlTheory.generic_app_fn_location_def]
     \\ rw[]
     >- (
@@ -1656,29 +1090,29 @@ Theorem compile_exps_code_labels
     \\ fs[] \\ NO_TAC)
   \\ TRY (
     reverse PURE_CASE_TAC
-    \\ fs[clos_to_bvlTheory.mk_cl_call_def, assign_get_code_label_def, MAP_GENLIST, o_DEF, IS_SOME_EXISTS]
+    \\ fs[clos_to_bvlTheory.mk_cl_call_def, closLangTheory.assign_get_code_label_def, MAP_GENLIST, o_DEF, IS_SOME_EXISTS]
     \\ fs[SUBSET_DEF, PULL_EXISTS, MEM_GENLIST, clos_to_bvlTheory.generic_app_fn_location_def]
     \\ rw[]
     \\ simp[domain_init_code, clos_to_bvlTheory.num_stubs_def]
-    \\ fs[MEM_MAP, clos_to_bvlTheory.free_let_def, MEM_GENLIST] \\ rveq \\ fs[assign_get_code_label_def]
+    \\ fs[MEM_MAP, clos_to_bvlTheory.free_let_def, MEM_GENLIST] \\ rveq \\ fs[closLangTheory.assign_get_code_label_def]
     \\ NO_TAC)
   \\ TRY (
     fs[IS_SOME_EXISTS] \\ rveq \\ fs[]
     \\ CHANGED_TAC(fs[CaseEq"list"]) \\ rveq \\ fs[]
     \\ TRY (
-      CHANGED_TAC(fs[CaseEq"prod"]) \\ rpt(pairarg_tac \\ fs[]) \\ rveq \\ fs[assign_get_code_label_def]
+      CHANGED_TAC(fs[CaseEq"prod"]) \\ rpt(pairarg_tac \\ fs[]) \\ rveq \\ fs[closLangTheory.assign_get_code_label_def]
       \\ fs[SUBSET_DEF, PULL_EXISTS, MEM_MAP]
       \\ imp_res_tac clos_to_bvlTheory.compile_exps_SING \\ rveq \\ fs[] \\ rveq \\ rw[]
       \\ fs[clos_to_bvlTheory.build_aux_def, clos_to_bvlTheory.build_recc_lets_def]
       \\ rveq \\ fs[MEM_GENLIST, clos_to_bvlTheory.free_let_def,MEM_MAP, clos_to_bvlTheory.recc_Let0_def]
-      \\ fsrw_tac[DNF_ss][assign_get_code_label_def]
+      \\ fsrw_tac[DNF_ss][closLangTheory.assign_get_code_label_def]
       \\ metis_tac[] )
     \\ pairarg_tac \\ fs[]
     \\ pairarg_tac \\ fs[]
     \\ fsrw_tac[DNF_ss][SUBSET_DEF, PULL_EXISTS]
-    \\ simp[clos_to_bvlTheory.build_recc_lets_def, assign_get_code_label_def]
-    \\ fsrw_tac[DNF_ss][MEM_MAP, PULL_EXISTS, assign_get_code_label_def]
-    \\ simp[clos_to_bvlTheory.recc_Let0_def, assign_get_code_label_def]
+    \\ simp[clos_to_bvlTheory.build_recc_lets_def, closLangTheory.assign_get_code_label_def]
+    \\ fsrw_tac[DNF_ss][MEM_MAP, PULL_EXISTS, closLangTheory.assign_get_code_label_def]
+    \\ simp[clos_to_bvlTheory.recc_Let0_def, closLangTheory.assign_get_code_label_def]
     \\ rw[]
     \\ TRY ( rpt disj1_tac \\ qexists_tac`SUC (LENGTH v7)` \\ simp[] \\ NO_TAC )
     \\ fs[recc_Lets_code_labels]
@@ -1694,7 +1128,7 @@ Theorem compile_exps_code_labels
       \\ imp_res_tac clos_to_bvlTheory.compile_exps_LENGTH
       \\ fs[MAP2_MAP, MEM_MAP, UNCURRY]
       \\ fs[clos_to_bvlTheory.code_for_recc_case_def, SND_EQ_EQUIV]
-      \\ rveq \\ fs[assign_get_code_label_def, MEM_MAP, MEM_GENLIST] \\ rveq \\ fs[assign_get_code_label_def]
+      \\ rveq \\ fs[closLangTheory.assign_get_code_label_def, MEM_MAP, MEM_GENLIST] \\ rveq \\ fs[closLangTheory.assign_get_code_label_def]
       \\ fs[MEM_ZIP] \\ rveq \\ fs[]
       \\ fs[clos_to_bvlTheory.compile_exps_def] \\ rveq \\ fs[]
       \\ `MEM (EL n (c1 ++ c2)) (c1 ++ c2)` by (
@@ -1731,7 +1165,7 @@ Theorem bvl_get_code_labels_JumpList
   `∀n xs. bvl_get_code_labels (JumpList n xs) = BIGUNION (set (MAP bvl_get_code_labels xs))`
   (recInduct bvl_jumpTheory.JumpList_ind
   \\ rw[]
-  \\ rw[Once  bvl_jumpTheory.JumpList_def, assign_get_code_label_def]
+  \\ rw[Once  bvl_jumpTheory.JumpList_def, closLangTheory.assign_get_code_label_def]
   \\ fs[LENGTH_EQ_NUM_compute]
   \\ Q.ISPECL_THEN[`LENGTH xs DIV 2`,`xs`]
        ((fn th => CONV_TAC(RAND_CONV(ONCE_REWRITE_CONV[th]))) o SYM)TAKE_DROP
@@ -1762,7 +1196,7 @@ Theorem clos_get_code_labels_alt_free
   (recInduct clos_annotateTheory.alt_free_ind
   \\ rw[clos_annotateTheory.alt_free_def]
   \\ rpt(pairarg_tac \\ fs[])
-  \\ rw[] \\ fs[map_replicate, clos_annotateTheory.const_0_def, assign_get_code_label_def]
+  \\ rw[] \\ fs[map_replicate, clos_annotateTheory.const_0_def, closLangTheory.assign_get_code_label_def]
   \\ fs[SUBSET_DEF, PULL_EXISTS]
   \\ imp_res_tac clos_annotateTheory.alt_free_SING \\ fs[MEM_REPLICATE_EQ]
   \\ fs[MEM_MAP, PULL_EXISTS, FORALL_PROD, UNCURRY, clos_annotateTheory.HD_FST_alt_free]
@@ -1806,7 +1240,7 @@ Theorem clos_get_code_labels_chain_exps
    BIGUNION (set (MAP (clos_get_code_labels) es)) ∪
    IMAGE ((+) n) (count (LENGTH es) DELETE 0)`
   (recInduct clos_to_bvlTheory.chain_exps_ind
-  \\ rw[clos_to_bvlTheory.chain_exps_def, assign_get_code_label_def]
+  \\ rw[clos_to_bvlTheory.chain_exps_def, closLangTheory.assign_get_code_label_def]
   >- ( EVAL_TAC \\ simp[] )
   \\ simp[Once EXTENSION, PULL_EXISTS, MEM_MAP, ADD1]
   \\ rw[EQ_IMP_THM] \\ fs[]
@@ -1826,7 +1260,7 @@ Theorem clos_get_code_labels_code_locs
   >- ( rw[EXTENSION] \\ metis_tac[] )
   >- ( rw[EXTENSION] \\ metis_tac[] )
   >- ( rw[EXTENSION] \\ metis_tac[] )
-  >- ( Cases_on`op` \\ fs[assign_get_code_label_def] )
+  >- ( Cases_on`op` \\ fs[closLangTheory.assign_get_code_label_def] )
   >- (
     rw[EXTENSION]
     \\ PURE_TOP_CASE_TAC \\ fs[]
@@ -2060,7 +1494,7 @@ Theorem clos_get_code_labels_mk_Ticks[simp]
 Theorem clos_get_code_labels_remove_fvs[simp]
   `∀n es. MAP clos_get_code_labels (remove_fvs n es) = MAP clos_get_code_labels es`
   (recInduct clos_fvsTheory.remove_fvs_ind
-  \\ rw[clos_fvsTheory.remove_fvs_def] \\ fs[assign_get_code_label_def]
+  \\ rw[clos_fvsTheory.remove_fvs_def] \\ fs[closLangTheory.assign_get_code_label_def]
   \\ AP_TERM_TAC
   \\ AP_TERM_TAC
   \\ AP_TERM_TAC
@@ -3470,9 +2904,9 @@ Theorem compile_correct
     \\ conj_tac >- (
       reverse conj_tac
       >- (
-        simp[clos_to_bvlTheory.init_globals_def, assign_get_code_label_def]
+        simp[clos_to_bvlTheory.init_globals_def, closLangTheory.assign_get_code_label_def]
         \\ simp[clos_to_bvlTheory.partial_app_fn_location_def]
-        \\ simp[SUBSET_DEF, MEM_MAP, PULL_EXISTS, MEM_FLAT, MEM_GENLIST, assign_get_code_label_def, domain_init_code]
+        \\ simp[SUBSET_DEF, MEM_MAP, PULL_EXISTS, MEM_FLAT, MEM_GENLIST, closLangTheory.assign_get_code_label_def, domain_init_code]
         \\ conj_tac
         >- (
           rw[]
@@ -3510,11 +2944,11 @@ Theorem compile_correct
       >- (
         pop_assum mp_tac
         \\ simp[clos_to_bvlTheory.generate_generic_app_def]
-        \\ simp[assign_get_code_label_def, bvl_get_code_labels_def,
+        \\ simp[closLangTheory.assign_get_code_label_def, bvl_get_code_labels_def,
                 bvl_jumpTheory.Jump_def,
                 clos_to_bvlTheory.partial_app_fn_location_code_def]
         \\ simp[MEM_MAP, MEM_GENLIST, PULL_EXISTS, bvl_get_code_labels_JumpList]
-        \\ simp[assign_get_code_label_def, clos_to_bvlTheory.mk_cl_call_def]
+        \\ simp[closLangTheory.assign_get_code_label_def, clos_to_bvlTheory.mk_cl_call_def]
         \\ simp[MEM_MAP, PULL_EXISTS, MEM_GENLIST]
         \\ simp[clos_to_bvlTheory.generic_app_fn_location_def] )
       \\ qmatch_asmsub_abbrev_tac`EL _ ls = z`
@@ -3527,7 +2961,7 @@ Theorem compile_correct
       \\ simp[MEM_FLAT, Abbr`ls`, MEM_GENLIST, PULL_EXISTS,Abbr`z`]
       \\ simp[clos_to_bvlTheory.generate_partial_app_closure_fn_def]
       \\ rw[]
-      \\ fs[assign_get_code_label_def, MEM_MAP, MEM_GENLIST] \\ rveq \\ fs[assign_get_code_label_def] )
+      \\ fs[closLangTheory.assign_get_code_label_def, MEM_MAP, MEM_GENLIST] \\ rveq \\ fs[closLangTheory.assign_get_code_label_def] )
     \\ fs[clos_to_bvlTheory.compile_common_def]
     \\ rpt(pairarg_tac \\ fs[]) \\ rveq \\ fs[]
     \\ specl_args_of_then``clos_to_bvl$compile_prog``(Q.GENL[`max_app`,`prog`] compile_prog_code_labels)mp_tac
